cogent/examples/repeat/RepeatShallowTest.thy
@@ -2,9 +2,9 @@ theory RepeatShallowTest
   imports RepeatShallow
 begin
 
-section "@{term repeatatl} Validation"
+section "@{term repeatatm} Validation"
 
-subsection "Fold Break using @{term repeatatl}"
+subsection "Fold Break using @{term repeatatm}"
 
 fun fold_break :: "('a \<Rightarrow> bool) \<Rightarrow> ('b \<Rightarrow> 'a \<Rightarrow> 'a) \<Rightarrow> 'b list \<Rightarrow> 'a \<Rightarrow> 'a"
   where
@@ -18,103 +18,103 @@ lemma "f (fold_break f g xs acc) \<Longrightarrow> fold_break f g (xs @ ys) acc 
 
 fun my_fold_break :: "('a \<Rightarrow> 'c \<Rightarrow> bool) \<Rightarrow> ('b \<Rightarrow> 'a \<Rightarrow> 'c \<Rightarrow> 'a) \<Rightarrow> 'b list \<Rightarrow> 'a \<Rightarrow> 'c \<Rightarrow> 'a"
   where
-"my_fold_break f g xs acc obsv = prod.fst (repeatatl (length xs) (\<lambda>(a, _) (_, b). f a b) (\<lambda>(a, i) (xs, b). (g (xs ! i) a b, Suc i)) (acc, 0) (xs, obsv))"
+"my_fold_break f g xs acc obsv = prod.fst (repeatatm (length xs) (\<lambda>(a, _) (_, b). f a b) (\<lambda>(a, i) (xs, b). (g (xs ! i) a b, Suc i)) (acc, 0) (xs, obsv))"
 
 lemma my_fold_break_helper1:
   "\<lbrakk>n \<le> length xs; f' = (\<lambda>(a, _) (_, b). f a b); g' = (\<lambda>(a, i) (xs, b). (g (xs ! i) a b, Suc i));
-    \<not>f' (repeatatl n f' g' (acc, 0) (xs, obsv)) (xs, obsv)\<rbrakk>
-    \<Longrightarrow> prod.snd (repeatatl n f' g' (acc, 0) (xs, obsv)) = n"
+    \<not>f' (repeatatm n f' g' (acc, 0) (xs, obsv)) (xs, obsv)\<rbrakk>
+    \<Longrightarrow> prod.snd (repeatatm n f' g' (acc, 0) (xs, obsv)) = n"
   apply (induct n)
-   apply (simp add: repeatatl.simps)
+   apply (simp add: repeatatm.simps)
   apply (clarsimp split: prod.splits)
-  apply (insert repeatatl_not_stop_Suc)
+  apply (insert repeatatm_not_stop_Suc)
   apply (drule_tac x = f' in meta_spec)
   apply (drule_tac x = n in meta_spec)
   apply (drule_tac x = g' in meta_spec)
   apply (drule_tac x = "(acc, 0)" in meta_spec)
   apply (drule_tac x = "(xs, obsv)" in meta_spec)
   apply (rotate_tac -1, drule meta_mp, simp)
-  apply (frule_tac n = n and f = f' and g = g' in repeatatl_step; simp)
+  apply (frule_tac n = n and f = f' and g = g' in repeatatm_step; simp)
   apply (clarsimp split: prod.splits)
   done
 
 lemma my_fold_break_helper1':
   "\<lbrakk>n \<le> length xs;
-    \<not>(\<lambda>(a, _) (_, b). f a b) (repeatatl n (\<lambda>(a, _) (_, b). f a b) (\<lambda>(a, i) (xs, b). (g (xs ! i) a b, Suc i)) (acc, 0) (xs, obsv)) (xs, obsv)\<rbrakk>
-    \<Longrightarrow> prod.snd (repeatatl n (\<lambda>(a, _) (_, b). f a b) (\<lambda>(a, i) (xs, b). (g (xs ! i) a b, Suc i)) (acc, 0) (xs, obsv)) = n"
+    \<not>(\<lambda>(a, _) (_, b). f a b) (repeatatm n (\<lambda>(a, _) (_, b). f a b) (\<lambda>(a, i) (xs, b). (g (xs ! i) a b, Suc i)) (acc, 0) (xs, obsv)) (xs, obsv)\<rbrakk>
+    \<Longrightarrow> prod.snd (repeatatm n (\<lambda>(a, _) (_, b). f a b) (\<lambda>(a, i) (xs, b). (g (xs ! i) a b, Suc i)) (acc, 0) (xs, obsv)) = n"
   apply (rule my_fold_break_helper1; simp?)
   done
 
 lemma my_fold_break_helper2:
   "\<lbrakk>n \<le> length xs; f' = (\<lambda>(a, _) (_, b). f a b); g' = (\<lambda>(a, i) (xs, b). (g (xs ! i) a b, Suc i));
-    repeatatl n f' g' (acc, 0) (xs, obsv) = (x, m);
+    repeatatm n f' g' (acc, 0) (xs, obsv) = (x, m);
     \<not>f x obsv\<rbrakk>
-    \<Longrightarrow> repeatatl n f' g' (acc, 0) (xs @ ys, obsv) = (x, m)"
+    \<Longrightarrow> repeatatm n f' g' (acc, 0) (xs @ ys, obsv) = (x, m)"
   apply (induct n arbitrary: x m)
-   apply (simp add: repeatatl.simps)
+   apply (simp add: repeatatm.simps)
   apply (clarsimp split: prod.splits)
-  apply (insert repeatatl_not_stop_Suc)
+  apply (insert repeatatm_not_stop_Suc)
   apply (drule_tac x = f' in meta_spec)
   apply (drule_tac x = n in meta_spec)
   apply (drule_tac x = g' in meta_spec)
   apply (drule_tac x = "(acc, 0)" in meta_spec)
   apply (drule_tac x = "(xs, obsv)" in meta_spec)
   apply (rotate_tac -1, drule meta_mp, simp)
-  apply (frule_tac n = n and f = f' and g = g' in repeatatl_step; simp)
+  apply (frule_tac n = n and f = f' and g = g' in repeatatm_step; simp)
   apply (clarsimp split: prod.splits)
   apply (drule_tac x = x1 and y = x2 in meta_spec2)
   apply clarsimp
-  apply (subst repeatatl_step; clarsimp)
+  apply (subst repeatatm_step; clarsimp)
   apply (cut_tac n = n and f = f and g = g and acc = acc and obsv = obsv and xs = xs in my_fold_break_helper1'; simp)
   apply (simp add: nth_append)
   done
 
 lemma my_fold_break_helper2':
   "\<lbrakk>n \<le> length xs;
-    repeatatl n  (\<lambda>(a, _) (_, b). f a b) (\<lambda>(a, i) (xs, b). (g (xs ! i) a b, Suc i)) (acc, 0) (xs, obsv) = (x, m);
+    repeatatm n  (\<lambda>(a, _) (_, b). f a b) (\<lambda>(a, i) (xs, b). (g (xs ! i) a b, Suc i)) (acc, 0) (xs, obsv) = (x, m);
     \<not>f x obsv\<rbrakk>
-    \<Longrightarrow> repeatatl n (\<lambda>(a, _) (_, b). f a b) (\<lambda>(a, i) (xs, b). (g (xs ! i) a b, Suc i)) (acc, 0) (xs @ ys, obsv) = (x, m)"
+    \<Longrightarrow> repeatatm n (\<lambda>(a, _) (_, b). f a b) (\<lambda>(a, i) (xs, b). (g (xs ! i) a b, Suc i)) (acc, 0) (xs @ ys, obsv) = (x, m)"
   apply (rule my_fold_break_helper2; simp)
   done
 
 lemma my_fold_break_helper3:
   "\<lbrakk>n \<le> length xs; f' = (\<lambda>(a, _) (_, b). f a b); g' = (\<lambda>(a, i) (xs, b). (g (xs ! i) a b, Suc i));
-    repeatatl n f' g' (acc, 0) (xs, obsv) = (x, m);
+    repeatatm n f' g' (acc, 0) (xs, obsv) = (x, m);
     f x obsv\<rbrakk>
-    \<Longrightarrow> repeatatl n f' g' (acc, 0) (xs @ ys, obsv) = (x, m)"
+    \<Longrightarrow> repeatatm n f' g' (acc, 0) (xs @ ys, obsv) = (x, m)"
   apply (induct n arbitrary: x m)
-   apply (simp add: repeatatl.simps)
+   apply (simp add: repeatatm.simps)
   apply (clarsimp split: prod.splits)
-  apply (case_tac "f' (repeatatl n f' g' (acc, 0) (xs, obsv)) (xs, obsv)")
-   apply (drule_tac n = n and f = f' and g = g' and a = "(acc, 0)" and b = "(xs, obsv)" in repeatatl_step_stop_Suc; clarsimp)
+  apply (case_tac "f' (repeatatm n f' g' (acc, 0) (xs, obsv)) (xs, obsv)")
+   apply (drule_tac n = n and f = f' and g = g' and a = "(acc, 0)" and b = "(xs, obsv)" in repeatatm_step_stop_Suc; clarsimp)
    apply (drule_tac x = x and y = m in meta_spec2)
    apply (drule meta_mp; simp)
-   apply (subst repeatatl_step_stop_Suc; clarsimp split: prod.split)
+   apply (subst repeatatm_step_stop_Suc; clarsimp split: prod.split)
   apply (frule_tac n = n and f = f and g = g and acc = acc and xs = xs and obsv = obsv in my_fold_break_helper1[rotated -1], simp, simp, simp)
-  apply (frule_tac n = n and f = f' and g = g' and a = "(acc, 0)" and b = "(xs, obsv)" in repeatatl_step; clarsimp split: prod.split)
+  apply (frule_tac n = n and f = f' and g = g' and a = "(acc, 0)" and b = "(xs, obsv)" in repeatatm_step; clarsimp split: prod.split)
   apply (cut_tac f = f and g = g and xs = xs and acc = acc and obsv = obsv and x = x1 and m = n and n = n and ys = ys in  my_fold_break_helper2')
      apply simp
     apply simp
    apply simp
-  apply (subst repeatatl_step; clarsimp split: prod.split)
+  apply (subst repeatatm_step; clarsimp split: prod.split)
   apply (drule_tac x = x1 and y = n in meta_spec2; clarsimp)
   apply (simp add: nth_append)
   done
 
 lemma my_fold_break_helper3':
   "\<lbrakk>n \<le> length xs;
-    repeatatl n (\<lambda>(a, _) (_, b). f a b) (\<lambda>(a, i) (xs, b). (g (xs ! i) a b, Suc i)) (acc, 0) (xs, obsv) = (x, m);
+    repeatatm n (\<lambda>(a, _) (_, b). f a b) (\<lambda>(a, i) (xs, b). (g (xs ! i) a b, Suc i)) (acc, 0) (xs, obsv) = (x, m);
     f x obsv\<rbrakk>
-    \<Longrightarrow> repeatatl n (\<lambda>(a, _) (_, b). f a b) (\<lambda>(a, i) (xs, b). (g (xs ! i) a b, Suc i)) (acc, 0) (xs @ ys, obsv) = (x, m)"
+    \<Longrightarrow> repeatatm n (\<lambda>(a, _) (_, b). f a b) (\<lambda>(a, i) (xs, b). (g (xs ! i) a b, Suc i)) (acc, 0) (xs @ ys, obsv) = (x, m)"
   apply (rule_tac f = f in my_fold_break_helper3; simp)
   done
 
 lemma fold_break_my_fold_break_eq:
   "fold_break (\<lambda>a. f a obsv) (\<lambda>a b. g a b obsv) xs acc = my_fold_break f g xs acc obsv"
   apply (induct rule: rev_induct[where xs = xs])
-   apply (simp add: repeatatl.simps)
+   apply (simp add: repeatatm.simps)
   apply clarsimp
-  apply (cut_tac p = "repeatatl (length xs) (\<lambda>(a, _) (_, y). f a y) (\<lambda>(a, i) (xs, b). (g (xs ! i) a b, Suc i)) (acc, 0) (xs, obsv)" in surj_pair)
+  apply (cut_tac p = "repeatatm (length xs) (\<lambda>(a, _) (_, y). f a y) (\<lambda>(a, i) (xs, b). (g (xs ! i) a b, Suc i)) (acc, 0) (xs, obsv)" in surj_pair)
   apply (erule exE)+
   apply (rename_tac y m)
   apply (rule conjI; rule impI)
@@ -122,14 +122,14 @@ lemma fold_break_my_fold_break_eq:
      apply simp
     apply simp
    apply simp
-   apply (subst repeatatl_step_stop_Suc; clarsimp split: prod.splits)
+   apply (subst repeatatm_step_stop_Suc; clarsimp split: prod.splits)
   apply (frule_tac n = "length xs" and xs = xs and x = y and ys = "[x]" and m = m in my_fold_break_helper2'[rotated 1])
     apply simp
    apply simp                                                                                     
   apply (cut_tac n = "length xs" and xs = xs and f = f and g = g and acc = acc and obsv = obsv in my_fold_break_helper1'[rotated 1])
     apply simp
    apply simp
-  apply (subst repeatatl_step; clarsimp split: prod.splits)
+  apply (subst repeatatm_step; clarsimp split: prod.splits)
   done
 
 end
